examples/n_german/nMutual.thy
@@ -31,9 +31,12 @@ text \<open>There cannot be one state in exit and another in critical or exit.
   n[i] = E \<longrightarrow> (\<forall>j. i \<noteq> j \<longrightarrow> n[j] \<noteq> C \<and> n[j] \<noteq> E)
 \<close>
 definition invAux :: "nat \<Rightarrow> nat \<Rightarrow> formula" where
-  "invAux N i \<equiv> IVar (Para ''n'' i) =\<^sub>f Const E \<longrightarrow>\<^sub>f
+"invAux N i \<equiv> IVar (Para ''n'' i) =\<^sub>f Const E \<longrightarrow>\<^sub>f
+                forallFormExcl 
+          (\<lambda>j. \<not>\<^sub>f IVar (Para ''n'' j) =\<^sub>f Const C  \<and>\<^sub>f \<not>\<^sub>f IVar (Para ''n'' j) =\<^sub>f Const E) i N"  
+ (* "invAux N i \<equiv> IVar (Para ''n'' i) =\<^sub>f Const E \<longrightarrow>\<^sub>f
                 forallFormExcl (\<lambda>j. \<not>\<^sub>f IVar (Para ''n'' j) =\<^sub>f Const C) i N \<and>\<^sub>f
-                forallFormExcl (\<lambda>j. \<not>\<^sub>f IVar (Para ''n'' j) =\<^sub>f Const E) i N"
+                forallFormExcl (\<lambda>j. \<not>\<^sub>f IVar (Para ''n'' j) =\<^sub>f Const E) i N"*)
 
 text \<open>Try enter critical region
   n[i] = I \<rightarrow> n[i] := T
@@ -87,11 +90,16 @@ definition n_Idle_abs1 :: rule where
     chaos \<triangleright> assign (Ident ''x'', Const true)"
 
 definition n_Idle_abs2 :: "nat \<Rightarrow> rule" where
-  "n_Idle_abs2 M \<equiv>
+"n_Idle_abs2 M \<equiv>
+    (\<forall>\<^sub>fj. ((\<not>\<^sub>f IVar (Para ''n'' j) =\<^sub>f Const (enum ''control'' ''C''))\<and>\<^sub>f
+      (\<not>\<^sub>f IVar (Para ''n'' j) =\<^sub>f Const (enum ''control'' ''E'')))) M 
+   \<triangleright>
+    assign (Ident ''x'', Const (boolV True))"
+  (*"n_Idle_abs2 M \<equiv>
     (\<forall>\<^sub>fj. \<not>\<^sub>f IVar (Para ''n'' j) =\<^sub>f Const (enum ''control'' ''C'')) M \<and>\<^sub>f
     (\<forall>\<^sub>fj. \<not>\<^sub>f IVar (Para ''n'' j) =\<^sub>f Const (enum ''control'' ''E'')) M
    \<triangleright>
-    assign (Ident ''x'', Const (boolV True))"
+    assign (Ident ''x'', Const (boolV True))"*)
 
 subsection \<open>Individual tests\<close>
 
@@ -139,11 +147,15 @@ text \<open>Move to idle, strengthened:
 definition n_Idle2_ref :: "nat \<Rightarrow> nat \<Rightarrow> rule" where
   "n_Idle2_ref N i \<equiv>
     IVar (Para ''n'' i) =\<^sub>f Const E \<and>\<^sub>f
-    forallFormExcl (\<lambda>j. \<not>\<^sub>f IVar (Para ''n'' j) =\<^sub>f Const C) i N \<and>\<^sub>f
-    forallFormExcl (\<lambda>j. \<not>\<^sub>f IVar (Para ''n'' j) =\<^sub>f Const E) i N
+    forallFormExcl (\<lambda>j.( \<not>\<^sub>f IVar (Para ''n'' j) =\<^sub>f Const C)  \<and>\<^sub>f
+       \<not>\<^sub>f IVar (Para ''n'' j) =\<^sub>f Const E) i N
    \<triangleright>
     assign (Para ''n'' i, Const I) ||
     assign (Ident ''x'', Const true)"
+
+(*IVar (Para ''n'' i) =\<^sub>f Const E \<and>\<^sub>f
+    forallFormExcl (\<lambda>j. \<not>\<^sub>f IVar (Para ''n'' j) =\<^sub>f Const C) i N \<and>\<^sub>f
+    forallFormExcl (\<lambda>j. \<not>\<^sub>f IVar (Para ''n'' j) =\<^sub>f Const E) i N*)
 
 lemma n_Idle2Eq:
   "strengthenRule2 (invAux N i) (n_Idle i) = n_Idle2_ref N i"
@@ -160,4 +172,485 @@ lemma absIdle2:
   "M \<le> N \<Longrightarrow> absTransfRule M (n_Idle2_ref N i) = (if i \<le> M then n_Idle i else n_Idle_abs2 M)"
   unfolding n_Idle_def n_Idle_abs2_def n_Idle2_ref_def by auto
 
+definition rules :: "nat \<Rightarrow> rule set" where [simp]:
+  "rules N \<equiv> {r.
+    (\<exists>i. i \<le> N \<and> r = n_Try i) \<or>
+    (\<exists>i. i \<le> N \<and> r = n_Crit i) \<or>
+    (\<exists>i. i \<le> N \<and> r = n_Exit i) \<or>
+    (\<exists>i. i \<le> N \<and> r = n_Idle i) 
+   }"
+
+
+definition n_Trys::" nat\<Rightarrow>rule set" where 
+  "n_Trys N== oneParamCons N  n_Try"
+
+definition n_Crits::" nat\<Rightarrow>rule set" where 
+  "n_Crits N== oneParamCons N  n_Crit"
+
+definition n_Exits::" nat\<Rightarrow>rule set" where 
+  "n_Exits N== oneParamCons N  n_Exit"
+
+definition n_Idles::" nat\<Rightarrow>rule set" where 
+  "n_Idles N== oneParamCons N  n_Idle"
+
+definition rules' :: "nat \<Rightarrow> rule set" where [simp]:
+  "rules' N \<equiv>  (n_Trys N) \<union> (n_Crits N)  \<union>
+    (n_Exits N) \<union>
+    (n_Idles N) 
+   "
+lemma n_TrysIsSym:
+  "symProtRules' N (n_Trys N)"
+  using Try(1) n_Trys_def symParaRuleInfSymRuleSet by auto
+
+lemma n_CritsIsSym:
+  "symProtRules' N (n_Crits N)"
+  using n_Crits_def symCrit(1) symParaRuleInfSymRuleSet by auto 
+
+lemma n_ExitsIsSym:
+  "symProtRules' N (n_Exits N)"
+  using n_Exits_def symExit(1) symParaRuleInfSymRuleSet by auto 
+
+lemma n_IdlesIsSym:
+  "symProtRules' N (n_Idles N)"
+  using n_Idles_def symIdle(1) symParaRuleInfSymRuleSet by auto
+
+lemma rulesSym':
+  shows "symProtRules' N (rules' N)"
+  using n_CritsIsSym n_ExitsIsSym n_IdlesIsSym n_TrysIsSym rules'_def symProtRulesUnion by presburger
+    
+lemma rulesSym:
+  shows "symProtRules' N (rules N)"
+  proof (simp only: symProtRules'_def, (rule allI)+, rule impI)
+  fix p r
+  assume a1: "p permutes {x.   x \<le> N} \<and> r \<in> rules N"
+  show "\<exists>r'. r' \<in> rules N \<and> equivRule (applySym2Rule p r) r'"
+  proof -
+    have b1:
+     "(\<exists>i. i \<le> N \<and> r = n_Try i) \<or>
+      (\<exists>i. i \<le> N \<and> r = n_Crit i) \<or>
+      (\<exists>i. i \<le> N \<and> r = n_Exit i) \<or>
+      (\<exists>i. i \<le> N \<and> r = n_Idle i) "
+      using local.a1 by auto
+    moreover
+    {assume b1:"\<exists> i. i\<le>N\<and>r=n_Try  i"
+      from b1 obtain i where b1:"i\<le>N\<and>r=n_Try  i"
+        by blast
+      have "symParamRule N n_Try"
+        by (simp add: Try(1))
+        
+      have "\<exists>r'. r' \<in> rules N \<and> equivRule (applySym2Rule p r) r'"
+        apply(cut_tac b1,simp)
+        apply(rule_tac x=" (n_Try (p i))" in exI)
+        apply(rule conjI)
+        apply (metis (full_types) local.a1 mem_Collect_eq permutes_def)
+        using \<open>symParamRule N n_Try\<close> local.a1 symParamRule_def by auto
+       
+    }
+    moreover
+    {assume b1:"\<exists> i. i\<le>N\<and>r=n_Crit  i"
+      from b1 obtain i where b1:"i\<le>N\<and>r=n_Crit  i"
+        by blast
+     have "symParamRule N n_Crit"
+       using symCrit(1) by blast
+        
+        
+      have "\<exists>r'. r' \<in> rules N \<and> equivRule (applySym2Rule p r) r'"
+        apply(cut_tac b1,simp)
+        apply(rule_tac x=" (n_Crit (p i))" in exI)
+        apply(rule conjI)
+        apply (metis (full_types) local.a1 mem_Collect_eq permutes_def)
+        using \<open>symParamRule N n_Crit\<close> local.a1 symParamRule_def by auto
+       
+    }
+    moreover
+    {assume b1:"\<exists> i. i\<le>N\<and>r=n_Idle  i"
+      from b1 obtain i where b1:"i\<le>N\<and>r=n_Idle  i"
+        by blast
+      have "symParamRule N n_Idle"
+       using symIdle(1) by blast
+        
+        
+      have "\<exists>r'. r' \<in> rules N \<and> equivRule (applySym2Rule p r) r'"
+        apply(cut_tac b1,simp)
+        apply(rule_tac x=" (n_Idle (p i))" in exI)
+        apply(rule conjI)
+        apply (metis (full_types) local.a1 mem_Collect_eq permutes_def)
+        using \<open>symParamRule N n_Idle\<close> local.a1 symParamRule_def by auto
+       
+    }
+    moreover
+    {assume b1:"\<exists> i. i\<le>N\<and>r=n_Exit  i"
+      from b1 obtain i where b1:"i\<le>N\<and>r=n_Exit  i"
+        by blast
+      have "symParamRule N n_Exit"
+       using symExit(1) by blast
+        
+        
+      have "\<exists>r'. r' \<in> rules N \<and> equivRule (applySym2Rule p r) r'"
+        apply(cut_tac b1,simp)
+        apply(rule_tac x=" (n_Exit (p i))" in exI)
+        apply(rule conjI)
+        apply (metis (full_types) local.a1 mem_Collect_eq permutes_def)
+        using \<open>symParamRule N n_Exit\<close> local.a1 symParamRule_def by auto
+       
+    }
+    ultimately show "\<exists>r'. r' \<in> rules N \<and> equivRule (applySym2Rule p r) r'"
+      by blast
+  qed
+qed
+
+definition F::"((nat\<Rightarrow>formula)\<times>(nat\<Rightarrow>formula)) set" where [simp]:
+"F \<equiv> {(%i. IVar (Para ''n'' i) =\<^sub>f Const E,
+               (%j.  \<not>\<^sub>f IVar (Para ''n'' j) =\<^sub>f Const C  \<and>\<^sub>f \<not>\<^sub>f IVar (Para ''n'' j) =\<^sub>f Const E) )}"
+
+definition rules2 :: "nat \<Rightarrow>rule set" where [simp]:
+  "rules2 N \<equiv> {r.
+    (\<exists>i. i \<le> N \<and> r =   (n_Try i)) \<or>
+    (\<exists>i. i \<le> N \<and> r =   (n_Crit i)) \<or>
+    (\<exists>i. i \<le> N \<and> r =   (n_Exit i)) \<or>
+    (\<exists> f i. f \<in> F  \<and> i \<le> N \<and> r =   (strengthenRule2  (constrInvByExcl f i N) (n_Idle i)) )
+   }"
+
+definition n_Idle2s::" nat \<Rightarrow>rule set" where 
+  "n_Idle2s N==
+  \<Union>{S. \<exists>p. p\<in>F \<and> S =oneParamCons N  (%i. (strengthenRule2  (constrInvByExcl p i N) (n_Idle i)))}"
+
+definition rules2' :: "nat \<Rightarrow> rule set" where [simp]:
+  "rules2' N \<equiv>  (n_Trys N) \<union> (n_Crits N)  \<union>
+    (n_Exits N) \<union>
+    (n_Idle2s N) "
+
+lemma rule2IsSym:
+  shows " symProtRules' N (rules2 N)" 
+  sorry
+axiomatization  where axiomOnf2 [simp,intro]:
+   "s  (Para ( ''n'') i) = I \<or> s  (Para ( ''n'') i) = T
+  \<or>s  (Para ( ''n'') i) = C \<or>s  (Para ( ''n'') i) = E"
+ 
+(*lemma False
+proof -
+  let ?s="(\<lambda>_. dontCare)(Para ''n'' 0 := enum ''control'' ''A'')"
+  have "?s(Para ''n'' 0) = enum ''control'' ''A''"
+    by auto
+  then show ?thesis
+    using axiomOnf2 by auto
+qed*)
+lemma symPreds:
+  shows "symPredSet' N ({initSpec0 N} Un { initSpec1})"
+proof -
+  let ?f="\<lambda> j . (\<forall>\<^sub>fi. IVar (Para ''n'' i) =\<^sub>f Const I) N"
+  let ?S1="oneParamFormCons N ?f"
+  have "{initSpec0 N}=?S1"
+    
+    using initSpec0_def oneParamFormCons_def  by auto
+
+  have "symPredSet' N ?S1" thm symParamFormForall
+    apply(rule  symParaFormInfSymFormSet) 
+    apply(rule symParamFormForall)
+    apply(unfold symParamForm2_def)
+    apply(unfold  equivForm_def,auto)
+    done
+    
+  have "symPredSet' N ({initSpec0 N})"
+    using \<open>symPredSet' N (oneParamFormCons N (\<lambda>j. (\<forall>\<^sub>fi. IVar (Para ''n'' i) =\<^sub>f Const I) N))\<close>
+      \<open>{initSpec0 N} = oneParamFormCons N (\<lambda>j. (\<forall>\<^sub>fi. IVar (Para ''n'' i) =\<^sub>f Const I) N)\<close> by auto
+
+  let ?f="\<lambda> j. IVar (Ident ''x'') =\<^sub>f Const true"
+  let ?S1="oneParamFormCons N ?f" 
+  have "{initSpec1 }=?S1"
+    
+    using initSpec1_def oneParamFormCons_def  by auto
+
+  have "symPredSet' N ?S1" thm symParamFormForall
+    apply(rule  symParaFormInfSymFormSet)  
+    apply(unfold symParamForm_def)
+    apply(unfold  equivForm_def,auto)
+    done
+
+  have "symPredSet' N ({initSpec1})"
+    using \<open>symPredSet' N (oneParamFormCons N (\<lambda>j. IVar (Ident ''x'') =\<^sub>f Const true))\<close> 
+      \<open>{initSpec1} = oneParamFormCons N (\<lambda>j. IVar (Ident ''x'') =\<^sub>f Const true)\<close> by auto
+  show "symPredSet' N ({initSpec0 N} \<union> {initSpec1})"
+    using \<open>symPredSet' N {initSpec0 N}\<close> \<open>symPredSet' N {initSpec1}\<close> symPredsUnion by blast
+qed
+
+definition absRules :: " rule set" where [simp]:
+  "absRules \<equiv> {r.
+    (\<exists>i. i \<le> 1 \<and> r = n_Try i) \<or>
+    (\<exists>i. i \<le> 1 \<and> r = n_Crit i) \<or>
+    (\<exists>i. i \<le> 1 \<and> r = n_Exit i) \<or>
+    (\<exists>i. i \<le> 1 \<and> r = n_Idle i) 
+   }\<union>{n_Idle_abs2 1}\<union>{n_Crit_abs } \<union> {chaos \<triangleright> skip} "
+
+
+lemma absRulesRef:
+  assumes a:"1 <N" and b:"M=1"
+  shows "absRules = {r'. \<exists>r. r \<in> rules2 N \<and> r' = absTransfRule M r}"
+proof
+  show "absRules \<subseteq> {r'. \<exists>r. r \<in> rules2 N \<and> r' = absTransfRule M r}"
+  proof
+    fix r
+    assume a1:"r\<in>absRules"
+    have "(\<exists>i. i \<le> M \<and> r = n_Try i) \<or>
+    (\<exists>i. i \<le> M \<and> r = n_Crit i) \<or>
+    (\<exists>i. i \<le> M \<and> r = n_Exit i) \<or>
+    (\<exists>i. i \<le> M \<and> r = n_Idle i) \<or>
+    (r=n_Idle_abs2 M)\<or>  r=n_Crit_abs |r= (chaos \<triangleright> skip)"
+      apply(cut_tac a1 b,unfold absRules_def,auto)done
+    moreover
+    {assume b1:"\<exists>i. i \<le> 1 \<and> r = n_Try i"
+      from b1 obtain i where b2:"i \<le> 1 \<and> r = n_Try i"
+        by blast
+      have "\<exists>r0. r0 \<in> rules2 N \<and> r = absTransfRule M r0"
+      apply(cut_tac b2,rule_tac x="r" in exI,simp,rule conjI)
+        apply (metis One_nat_def a le_trans less_imp_le)
+         
+        by (simp add: Try(3) b)
+    } 
+    moreover
+    {assume b1:"r=n_Idle_abs2 M"
+      let ?f="(%i. IVar (Para ''n'' i) =\<^sub>f Const E,
+               (%j.  \<not>\<^sub>f IVar (Para ''n'' j) =\<^sub>f Const C  \<and>\<^sub>f \<not>\<^sub>f IVar (Para ''n'' j) =\<^sub>f Const E) )" 
+      have "\<exists>r0. r0 \<in> rules2 N \<and> r = absTransfRule M r0"
+      apply( rule_tac x="(strengthenRule2  (constrInvByExcl ?f 2 N) (n_Idle 2))" in exI,simp,rule conjI)
+
+      apply (metis One_nat_def a add.right_neutral add_Suc_right not_less not_less_eq_eq one_add_one)
+        using a absIdle2 b b1 invAux_def n_Idle2Eq by auto
+      
+    } 
+    moreover
+    {assume b1:"\<exists>i. i \<le> 1 \<and> r = n_Crit i"
+      from b1 obtain i where b2:"i \<le> 1 \<and> r = n_Crit i"
+        by blast
+      have "\<exists>r0. r0 \<in> rules2 N \<and> r = absTransfRule M r0"
+      apply(cut_tac b2,rule_tac x="r" in exI,simp,rule conjI)
+        apply (metis One_nat_def a le_trans less_imp_le)
+        by (simp add: b symCrit(3))
+    }
+   moreover
+   {assume b1:"\<exists>i. i \<le> 1 \<and> r = n_Idle i"
+      from b1 obtain i where b2:"i \<le> 1 \<and> r = n_Idle i"
+        by blast
+      let ?f="(%i. IVar (Para ''n'' i) =\<^sub>f Const E,
+               (%j.  \<not>\<^sub>f IVar (Para ''n'' j) =\<^sub>f Const C  \<and>\<^sub>f \<not>\<^sub>f IVar (Para ''n'' j) =\<^sub>f Const E) )" 
+      have "\<exists>r0. r0 \<in> rules2 N \<and> r = absTransfRule M r0"
+      apply(rule_tac x="(strengthenRule2  (constrInvByExcl ?f i N) (n_Idle i))" in exI,simp,rule conjI)
+      apply (smt a b2 le_trans less_imp_le)
+        using a absIdle2 b b2 invAux_def n_Idle2Eq by auto    
+    }
+     moreover
+    {assume b1:"\<exists>i. i \<le> 1 \<and> r = n_Exit i"
+      from b1 obtain i where b2:"i \<le> 1 \<and> r = n_Exit i"
+        by blast
+      have "\<exists>r0. r0 \<in> rules2 N \<and> r = absTransfRule M r0"
+      apply(cut_tac b2,rule_tac x="r" in exI,simp,rule conjI)
+        apply (metis One_nat_def a le_trans less_imp_le)
+        by (simp add: b symExit(3))
+    }
+    moreover
+    {assume b1:"r=n_Crit_abs"
+       have "\<exists>r0. r0 \<in> rules2 N \<and> r = absTransfRule M r0"
+      apply( rule_tac x="  (n_Crit 2) " in exI,simp,rule conjI)
+
+      apply (metis One_nat_def a add.right_neutral add_Suc_right not_less not_less_eq_eq one_add_one)
+         by (simp add: b b1 symCrit(3))
+        
+      
+    }
+     moreover
+    {assume b1:"r=(chaos \<triangleright> skip)"
+     have "\<exists>r0. r0 \<in> rules2 N \<and> r = absTransfRule M r0"
+      apply( rule_tac x="  (n_Try 2) " in exI,simp,rule conjI)
+
+      apply (metis One_nat_def a add.right_neutral add_Suc_right not_less not_less_eq_eq one_add_one)
+       by (simp add: Try(3) b b1) 
+   }
+   ultimately show "r \<in>{r. \<exists>r0. r0 \<in> rules2 N \<and> r = absTransfRule M r0}"
+     using b by blast
+ qed
+ next
+   show  "{r'. \<exists>r. r \<in> rules2 N \<and> r' = absTransfRule M r} \<subseteq> absRules"
+   proof
+     fix x
+     assume b1:" x \<in> {r'. \<exists>r. r \<in> rules2 N \<and> r' = absTransfRule M r}"
+     have "(\<exists>i. i \<le> N \<and> x = absTransfRule M  (n_Try i)) \<or>
+    (\<exists>i. i \<le> N \<and> x = absTransfRule M  (n_Crit i)) \<or>
+    (\<exists>i. i \<le> N \<and> x =  absTransfRule M (n_Exit i)) \<or>
+    (\<exists> f i. f \<in> F  \<and> i \<le> N \<and>
+       x = absTransfRule M  (strengthenRule2  (constrInvByExcl f i N) (n_Idle i)) )
+   "
+       using b1 by auto
+     moreover
+     {assume b1:"(\<exists>i. i \<le> N \<and> x = absTransfRule M  (n_Try i))"
+       from b1 obtain i where b2:"i \<le> N \<and> x = absTransfRule M  (n_Try i)"
+         by blast
+         have "x \<in> absRules"
+           apply(case_tac "i \<le>M")
+           using Try(3) b b2 apply auto[1]
+           by (simp add: Try(3) b2)
+       }
+      moreover
+     {assume b1:"(\<exists>i. i \<le> N \<and> x = absTransfRule M  (n_Exit i))"
+       from b1 obtain i where b2:"i \<le> N \<and> x = absTransfRule M  (n_Exit i)"
+         by blast
+         have "x \<in> absRules"
+           apply(case_tac "i \<le>M")
+           using b b2 symExit(3) apply auto[1] 
+           by (simp add: symExit(3) b2)
+       }
+     moreover
+     {assume b1:"(\<exists>i. i \<le> N \<and> x = absTransfRule M  (n_Crit i))"
+       from b1 obtain i where b2:"i \<le> N \<and> x = absTransfRule M  (n_Crit i)"
+         by blast
+         have "x \<in> absRules"
+           apply(case_tac "i \<le>M")
+           using b b2 symCrit(3) apply auto[1] 
+           by (simp add: symCrit(3) b2)
+       }
+      moreover
+     {assume b1:"(\<exists> f i. f \<in> F  \<and> i \<le> N \<and> x = absTransfRule M  (strengthenRule2  (constrInvByExcl f i N) (n_Idle i)) )"
+       from b1 obtain f i where b2:"f \<in> F  \<and>i \<le> N \<and> 
+      x = absTransfRule M (strengthenRule2  (constrInvByExcl f i N) (n_Idle i)) "
+         by blast
+       have "x \<in> absRules"
+         proof(case_tac "i \<le>M")
+           assume c1:"i\<le>M"
+           have c2:"x= n_Idle i" 
+           apply(cut_tac b2 c1,unfold n_Idle_def,auto ) 
+             done
+           show "x \<in> absRules"
+             using b c1 c2 by auto
+         next
+           assume c1:"~i\<le>M"
+           have c2:"x=n_Idle_abs2 M " 
+             by(cut_tac b2 c1,unfold n_Idle_def  n_Idle_abs2_def,auto )  
+            show "x \<in> absRules"
+             using b c1 c2 by auto
+         qed    
+       }
+       ultimately  show "x \<in> absRules"
+         by blast
+     qed
+   qed
+
+axiomatization  where axiomOnAbsProt [simp,intro]:
+   "\<forall>i f s.
+       f \<in> F \<longrightarrow>
+       reachableUpTo {f'. \<exists>f. f \<in> {initSpec0 N} \<union> {initSpec1} \<and> f' = absTransfForm M f}
+        absRules i s \<longrightarrow>
+       formEval (constrInv f 0 1) s"
+
+lemma absProtSim:
+  assumes (*a1:"F= {(%i. IVar (Para ''n'' i) =\<^sub>f Const E,
+               (%j.  \<not>\<^sub>f IVar (Para ''n'' j) =\<^sub>f Const C  \<and>\<^sub>f \<not>\<^sub>f IVar (Para ''n'' j) =\<^sub>f Const E) )}" 
+    and*) a2:"M<N" and a3:"M=1"
+  shows "\<forall>f s. f\<in>constrInvByExcls F  N \<longrightarrow> 
+  reachableUpTo  ({initSpec0 N} Un { initSpec1}) (rules N) i s \<longrightarrow> formEval f s"
+proof(rule_tac ?rs2.0="rules2 N" in   CMP)
+  show " \<And>r. r \<in> rules N \<longrightarrow> wellFormedRule N r"
+  proof(rule impI)
+    fix r
+    assume b1:"r \<in> rules N"
+    have " (\<exists>i. i \<le> N \<and> r= n_Try i)\<or>(\<exists>i. i \<le> N  \<and> r= n_Crit i)\<or>
+      (\<exists>i. i \<le> N \<and>r= n_Exit i)\<or>(\<exists>i. i \<le> N \<and>r=n_Idle i)"
+      apply(cut_tac b1,auto)done
+    moreover
+    {assume b1:"\<exists>i. i \<le> N \<and> r= n_Try i"
+      from b1 obtain i where b1:"i \<le> N \<and> r= n_Try i"
+        by blast
+        have "wellFormedRule N r"
+          by (metis Try(2) act.simps b1 wellFormedRule.elims(3))
+      }  
+
+    moreover
+    {assume b1:"\<exists>i. i \<le> N \<and> r= n_Crit i"
+      from b1 obtain i where b1:"i \<le> N \<and> r= n_Crit i"
+        by blast
+       have "wellFormedRule N r"
+         by (metis act.simps b1 symCrit(2) wellFormedRule.elims(3)) 
+     } 
+
+    moreover
+    {assume b1:"\<exists>i. i \<le> N \<and> r= n_Idle i"
+      from b1 obtain i where b1:"i \<le> N \<and> r= n_Idle i"
+        by blast
+       have "wellFormedRule N r"
+               
+         by (metis act.simps b1 symIdle(2) wellFormedRule.elims(3))
+     }  
+
+     moreover
+    {assume b1:"\<exists>i. i \<le> N \<and> r= n_Exit i"
+      from b1 obtain i where b1:"i \<le> N \<and> r= n_Exit i"
+        by blast
+       have "wellFormedRule N r"
+         by (metis act.simps b1 symExit(2) wellFormedRule.elims(3))
+               
+     
+     }  
+     ultimately show "wellFormedRule N r"
+       by auto
+   qed
+ next
+   show "\<forall>f. f \<in> F \<longrightarrow> symPair f N"
+   proof(rule allI,rule impI)
+     fix f
+     assume c1:"f \<in> F"
+     show "symPair f N"
+       apply(cut_tac a1 c1,simp) 
+       apply(rule conjI)
+       apply(unfold symParamForm_def)
+       apply((rule allI)+,(rule impI)+)
+        apply(unfold equivForm_def,force)
+       apply((rule allI)+,(rule impI)+)
+       apply(force)
+       done
+   qed
+ next
+ 
+next
+  show "symProtRules' N (rules N)"
+    using rulesSym by blast
+next
+  show "symPredSet' N ({initSpec0 N} \<union> {initSpec1})"
+    using symPreds by blast
+
+next
+  show "M \<le> N"
+    apply (cut_tac  a2,arith) done
+next
+  show " \<forall>s f. f \<in> F \<longrightarrow> (\<forall>v. v \<in> varOfForm (constrInv f 0 1) \<longrightarrow> s v = abs1 M s v)"
+    apply(cut_tac  a3, simp,auto)
+    using axiomOnf2 apply force
+    using axiomOnf2 apply force
+    done
+next
+  show "\<forall>r'. r' \<in> rules2 N \<longrightarrow>
+         (\<exists>r f i. f \<in> F \<and> r \<in> rules N \<and> i \<le> N  \<and> r' = strengthenRule2 (constrInvByExcl f i N) r) \<or>
+         r' \<in> rules N"
+    apply(unfold rules2_def rules_def)
+    apply auto
+    done
+next
+  show " symProtRules' N (rules2 N)"
+    using rule2IsSym by blast 
+next
+  show " \<forall>r. r \<in> rules N \<longrightarrow> (\<exists>f. f \<in> constrInvByExcls F N \<and> strengthenRule2 f r \<in> rules2 N)
+   \<or> r \<in> rules2 N"
+  apply(unfold rules2_def rules_def)
+    apply auto
+    done
+next 
+  show "1 \<le> N"
+    using a2 a3 by arith
+  
+next 
+  show "\<forall>i f s.
+       f \<in> F \<longrightarrow>
+       reachableUpTo {f'. \<exists>f. f \<in> {initSpec0 N} \<union> {initSpec1} \<and> f' = absTransfForm M f}
+        {r'. \<exists>r. r \<in> rules2 N \<and> r' = absTransfRule M r} i s \<longrightarrow>
+       formEval (constrInv f 0 1) s"
+  
+    using a2 a3 absRulesRef axiomOnAbsProt by auto
+qed
 end
